Rename node_replication

examples/node_replication.v
@@ -1,6 +1,3 @@
-(* Lambda calculus with the call-by-need reduction strategy *)
-(* version of Danvy & Zerny PPDP13, 'revised cbneed λ_let-calculus of Fig. 5 *)
-
 Require Import Program.
 Require Import Util.
 Require Import refocusing_semantics.
@@ -14,15 +11,6 @@ Require Import Sets.
 (* The module type PRE_RED_SEM is defined in the file *)
 (*     reduction_semantics/reduction_semantics.v *)
 (* It is a RED_SEM without totality of decompose *)
-
-Ltac assert_by_proof_irrelevance :=
-  match goal with
-  | [ H : ?P, H1 : ?P |- _  ] => assert (H=H1) by apply proof_irrelevance
-  end.
-
-Ltac subst_proof_irrelevance := assert_by_proof_irrelevance; subst.
-Ltac dep_subst_proof_irrelevance := assert_by_proof_irrelevance; dep_subst.
-
 
 Module Lam_cbnd_PreRefSem <: PRE_RED_SEM.
 
@@ -53,18 +41,10 @@ Module Lam_cbnd_PreRefSem <: PRE_RED_SEM.
 
   (* Weak call-by-need is a uniform strategy, so one context kind E is enough. *)
 
-  Inductive ck := N.
+  Inductive ck := E.
 
-  Inductive ckvar : Type :=
-  | ckv : ck -> var -> ckvar.
-
-  Definition ckind := ckvar.
+  Definition ckind := ck.
   Hint Unfold  ckind.
-
-  (* Here we define the language of interest: lambda-let calculus.  *)
-  (* Needys parameterized by a variable x are evaluation contexts *)
-  (* with x plugged in the hole. Thus they are neutral terms with *)
-  (* the variable x being needed. *)
 
   Inductive expr :=
   | Var       : var -> expr                                 (* variable *)
@@ -105,12 +85,28 @@ Module Lam_cbnd_PreRefSem <: PRE_RED_SEM.
   Definition term := expr.
   Hint Unfold term.
 
+  Fixpoint fresh_ind_n {x} (nx : needy x) : nat :=
+    match nx with
+    | nVar (Id x) => x
+    | nApp _ nx t => max (fresh_ind_n nx) (fresh_ind t)
+    | nExpSubst (Id x) (Id y) _ nx u => max (max (max (fresh_ind_n nx) (fresh_ind u)) y) x
+    | nExpSubstS (Id x) (Id y) nx ny => max (max (max (fresh_ind_n nx) (fresh_ind_n ny)) y) x
+    | nExpDist (Id x) (Id y) (Id z) _ nx u => max (max (max (max (fresh_ind_n nx) (fresh_ind u)) z) y) x
+    end
+  with fresh_ind (t : term) : nat :=
+    match t with
+    | Var (Id x) => x
+    | Lam (Id x) p => max (fresh_ind p) x
+    | App p q => max (fresh_ind p) (fresh_ind q)
+    | ExpSubst p (Id x) u => max (max (fresh_ind p) (fresh_ind u)) x
+    | ExpSubstS (Id x) nx u => max (max (fresh_ind u) (fresh_ind_n nx)) x
+    | ExpDist p (Id x) (Id y) u =>
+        max (max (fresh_ind p) (fresh_ind u)) (max x y)
+    | ExpDistS (Id x) nx (Id y) u =>
+        max (max (fresh_ind_n nx) (fresh_ind u)) (max x y)
+    end.
 
-  (* L - Lists context *)
-  Inductive ansCtx : ckind -> Type :=
-  | ansCtxEmpty : forall {k}, ansCtx k                                  (* <> *)
-  | ansCtxSubst : forall {k}, ansCtx k -> var -> term -> ansCtx k         (* L[x / u] *)
-  | ansCtxDist  : forall {k}, ansCtx k -> var -> var -> term -> ansCtx k. (* L[x // λy.u] *)
+  Definition fresh_var t := Id (fresh_ind t).
 
   (* L - Lists context *)
   Inductive sub :=
@@ -126,7 +122,6 @@ Module Lam_cbnd_PreRefSem <: PRE_RED_SEM.
     | subDist s' x y r => ExpDist (sub_to_term s' t) x y r
     end.
 
-  (* v *)
   Inductive val : ckind -> Type :=
   | vLam : forall {k}, var -> term -> val k.
 
@@ -138,33 +133,11 @@ Module Lam_cbnd_PreRefSem <: PRE_RED_SEM.
   Coercion val_to_term : val >-> term.
 
   Inductive answer : ckind -> Type :=
-  | ansVal : forall {k}, val k -> sub -> answer k
-  | ansNd : forall {k} x, needy x -> answer k.
+  | ansVal : val E -> sub -> answer E
+  | ansNd : forall x, needy x -> answer E.
 
-  (* It should be made clear here that the values in this *)
-  (* implementation of refocusing are not the same as values in the Danvy *)
-  (* and Zerny's paper. The implementation requires all useful normal forms *)
-  (* to be values. By "useful" we mean that such a normal form put into *)
-  (* some reduction context does participate in further computation. Stuck *)
-  (* term thtat remain stuck in all reduction contexts need not be *)
-  (* values. *)
-
-
-
-  (* In this setting needys cannot be stuck terms. Needys are *)
-  (* intermediate values and we have to treat them as values *)
-  (* Hence the category of values mast contain both answers  *)
-  (* and needys *)
   Definition value := answer.
   Hint Unfold value.
-
-  (* A function for plugging a term to an answer context *)
-  Fixpoint ansCtx_plug {k} (s : ansCtx k) (t : term) :=
-  match s with
-  | ansCtxEmpty => t
-  | ansCtxSubst s' x r => ExpSubst (ansCtx_plug s' t) x r
-  | ansCtxDist s' x y r => ExpDist (ansCtx_plug s' t) x y r
-  end.
 
   (* A function for plugging a term to an answer context *)
   Fixpoint sub_plug (s : sub) (t : term) :=
@@ -173,14 +146,6 @@ Module Lam_cbnd_PreRefSem <: PRE_RED_SEM.
   | subSubst s' x r => ExpSubst (sub_plug s' t) x r
   | subDist s' x y r => ExpDist (sub_plug s' t) x y r
   end.
-
-  Fixpoint sub_to_ansCtx {k} (s : sub) : ansCtx k :=
-    match s with
-    | subEmpty => ansCtxEmpty
-    | subSubst s' x r => ansCtxSubst (sub_to_ansCtx s') x r
-    | subDist s' x y r => ansCtxDist (sub_to_ansCtx s') x y r
-    end.
-
 
   Fixpoint needy_to_term {x} (n : needy x) : term :=
   match n with
@@ -202,45 +167,27 @@ Module Lam_cbnd_PreRefSem <: PRE_RED_SEM.
   Coercion answer_to_term : answer >-> term.
   Coercion needy_to_term : needy >-> term.
 
-  (* Here we define the set of potential redices. *)
-  (* Actually, they are just redices as defined in the paper *)
-  (* Inductive red : ckind -> Type := *)
-  (* | rApp  : forall {k} {n:nat}, ansCtx k -> val k -> term -> red k        (1* L<v> u *1) *)
-  (* | rSplS : forall {k} (n:nat) x, needy x -> val k -> ansCtx k -> red k   (1* N<<x>>[[x/L<λy.p>]] *1) *)
-  (* | rSpl  : forall {k} {n:nat} x, needy x -> term -> red k                (1* N<<x>>[x/t] *1) *)
-  (* | rLsS  : forall {k} {n:nat} x, needy x -> val k -> red k               (1* N<<x>>[[x//v]] *1) *)
-  (* | rLs   : forall {k} {n:nat} x, needy x -> val k -> red k.              (1* N<<x>>[x//t] *1) *)
-
-
-
-
-(* Here we define the set of potential redices. *)
+ (* Here we define the set of potential redices. *)
  (* Actually, they are just redices as defined in the paper *)
  Inductive red : ckind -> Type :=
  | rApp  : forall {k}, val k -> sub -> term -> red k (* L<λx.u> t *)
  | rSplS : forall {k} x, needy x -> val k -> sub -> red k (* N<<x>>[[x/L<λy.p>]] *)
- | rSpl  : forall {k} x, needy x -> term -> red k                (* N<<x>>[x/t] *)
- | rLsS  : forall {k} x, needy x -> val k -> red k               (* N<<x>>[[x//v]] *)
- | rLs   : forall {k} x, needy x -> val k -> red k.              (* N<<x>>[x//v] *)
- (* TODO  check "val k" vs. "val (ckv k z)". the same for ansCtx *)
-
-  (* Daniel: redices for `activations':
-      + N<<x>>[x/t]  -> N<<x>>[[x/t]]
-      + N<<x>>[x//t] -> N<<x>>[[x//t]]
-   *)
+ | rSpl  : forall {k} x, needy x -> term -> red k         (* N<<x>>[x/t] *)
+ | rLsS  : forall {k} x, needy x -> val k -> red k        (* N<<x>>[[x//v]] *)
+ | rLs   : forall {k} x, needy x -> val k -> red k.       (* N<<x>>[x//v] *)
 
   Definition redex := red.
   Hint Unfold redex.
 
 
   Definition redex_to_term {k} (r : redex k) : term :=
-      match r with
-      | rApp v l t => App (sub_to_term l (val_to_term v)) t
-      | rSplS x n v s => ExpSubstS x n (sub_to_term s (val_to_term v))
-      | rSpl x n t => ExpSubst (needy_to_term n) x t
-      | rLsS x n (vLam y t) => ExpDistS x n y t
-      | rLs x n (vLam y t) => ExpDist (needy_to_term n) x y t
-      end.
+    match r with
+    | rApp v l t => App (sub_to_term l (val_to_term v)) t
+    | rSplS x n v s => ExpSubstS x n (sub_to_term s (val_to_term v))
+    | rSpl x n t => ExpSubst (needy_to_term n) x t
+    | rLsS x n (vLam y t) => ExpDistS x n y t
+    | rLs x n (vLam y t) => ExpDist (needy_to_term n) x y t
+    end.
 
   Coercion redex_to_term : redex >-> term.
 
@@ -250,64 +197,6 @@ Module Lam_cbnd_PreRefSem <: PRE_RED_SEM.
   Proof with eauto.
     destruct v. intros. dependent destruction v'. inversion H.
     reflexivity.
-  Qed.
-
-
-  Lemma ansCtx_plug_val_injective :
-    forall {k} (s s' : ansCtx k) (v v' : val k),
-    ansCtx_plug s v = ansCtx_plug s' v' -> s = s' /\ v = v'.
-  Proof with auto.
-    intros k s s' v v' H.
-    induction s; dependent destruction s'; inversion H.
-    destruct v; dependent destruction v'; inversion H1...
-    destruct v0; dependent destruction s'; inversion H1...
-    destruct v1; dependent destruction s'; inversion H1...
-    destruct v; dependent destruction v'; inversion H1...
-    split; f_equal; elim IHs with s' v1 v'...
-    dependent destruction s; destruct v'; inversion H1; split...
-    split; f_equal; elim IHs with s' v3 v'...
-  Qed.
-
-
-  Lemma ansCtx_plug_var_injective :
-    forall {k} (s s' : ansCtx k) x x',
-    ansCtx_plug s (Var x) = ansCtx_plug s' (Var x') -> s = s' /\ x = x'.
-  Proof with auto.
-    intros k s s' x x' H.
-    induction s; dependent destruction s'; inversion H...
-    split; f_equal; elim IHs with s'...
-    split; f_equal; elim IHs with s'...
-  Qed.
-
-
-  Lemma ansCtx_plug_needy :
-    forall {k} (s s' : ansCtx k) (v : val k) {x} (n : needy x),
-    ansCtx_plug s v = ansCtx_plug s' n -> False.
-  Proof with auto.
-    induction s; simpl; intros.
-    destruct v; destruct s'; destruct n; discriminate.
-    destruct s'. destruct n; simpl in *; try discriminate.
-    inversion H; elim IHs with ansCtxEmpty v0 x n0...
-    inversion H; elim (IHs _ _ _ _ H1).
-    inversion H.
-    destruct s'. destruct n; simpl in *; try discriminate.
-    inversion H. elim IHs with ansCtxEmpty v1 x n0...
-    inversion H; elim (IHs _ _ _ _ H1).
-    inversion H; elim (IHs _ _ _ _ H1).
-  Qed.
-
-  Lemma ansCtx_plug_var :
-    forall {k} (s s' : ansCtx k) x (v : val k),
-    ansCtx_plug s v = ansCtx_plug s' (Var x) -> False.
-  Proof with auto.
-    induction s; simpl; intros.
-    destruct v; destruct s'; discriminate.
-    destruct s'. discriminate.
-    inversion H. elim IHs with s' x v0...
-    inversion H.
-    destruct s'. discriminate.
-    inversion H. elim IHs with s' x v1...
-    inversion H. elim IHs with s' x v1...
   Qed.
 
   Lemma sub_plug_needy :
@@ -339,10 +228,9 @@ Module Lam_cbnd_PreRefSem <: PRE_RED_SEM.
       dependent rewrite H0; auto.
     - elim IHn2 with n'2...
     - subst; rewrite proof_irrelevance with (x0 <> y) n n1...
- Qed.
+  Qed.
 
-
-Lemma sub_to_term_val_injective :
+  Lemma sub_to_term_val_injective :
     forall {k} (s s' : sub) (v v' : val k),
       sub_to_term s v = sub_to_term s' v' ->
       s = s' /\ v = v'.
@@ -356,9 +244,9 @@ Lemma sub_to_term_val_injective :
     elim IHs with s' v1 v'; intros; subst...
     destruct v1; dependent destruction v'; inversion H...
     elim IHs with s' v3 v'; intros; subst...
- Qed.
+  Qed.
 
-Lemma sub_to_term_var_injective :
+  Lemma sub_to_term_var_injective :
     forall (s s' : sub) x x',
       sub_to_term s (Var x) = sub_to_term s' (Var x') -> s = s' /\ x = x'.
   Proof with eauto.
@@ -368,30 +256,25 @@ Lemma sub_to_term_var_injective :
     elim IHs with s' x x'; intros; subst...
   Qed.
 
-(*DANIEL: based on strong lemmas *)
   Lemma answer_val_not_needy :
-  forall {k} (s: sub) (v : val k) t,
-      sub_to_term s v = t ->
-      forall {x} (n : needy x), t = needy_to_term n ->   False.
+    forall {k x} (s: sub) (v : val k) (n : needy x), sub_to_term s v = needy_to_term n -> False.
   Proof.
-   induction s; intros; dependent destruction v;
-   dependent destruction n; subst; try discriminate.
-  Admitted.
+   induction s; intros; dependent destruction n;
+   dependent destruction v; subst; try discriminate;
+   simpl in H; inversion H; eapply IHs; apply H1.
+  Qed.
 
   Lemma answer_to_term_injective :
     forall {k} (a a' : answer k),
     answer_to_term a = answer_to_term a' -> a = a'.
   Proof with auto.
-   dependent destruction a; dependent destruction  a'; intros; inversion H;
-      subst; repeat dep_subst_proof_irrelevance.
-    - f_equal; elim sub_to_term_val_injective with s s0 v v0...
-    - eelim answer_val_not_needy; eauto.
-    - eelim answer_val_not_needy; eauto.
-    - elim needy_to_term_injective with n n0; intros; subst...
-      rewrite H...
+   destruct a; dependent destruction  a'; intros...
+    f_equal; elim sub_to_term_val_injective with s s0 v v0...
+    eelim answer_val_not_needy; eauto.
+    eelim answer_val_not_needy; eauto.
+    elim needy_to_term_injective with n n0; intros; subst...
+    rewrite H0...
   Qed.
-
-
 
   Definition value_to_term {k} (a : value k) := answer_to_term a.
 
@@ -401,72 +284,57 @@ Lemma sub_to_term_var_injective :
     intros; apply answer_to_term_injective...
   Qed.
 
-
   Lemma redex_to_term_injective :
       forall {k} (r r' : redex k), redex_to_term r = redex_to_term r' -> r = r'.
-
   Proof with auto.
     intros k r r' H.
     destruct r; dependent destruction r';
     inversion H; subst.
     - eelim sub_to_term_val_injective; intros; eauto; subst; trivial.
-    - dependent destruction v; dependent destruction v0... inversion H.
-    - dependent destruction v; dependent destruction v0... inversion H.
+    - dependent destruction v; dependent destruction v0; inversion H.
+    - dependent destruction v; dependent destruction v0; inversion H.
     - eelim sub_to_term_val_injective; intros; eauto; subst; trivial.
-    - dependent destruction v; dependent destruction v0... inversion H.
-    - dependent destruction v; dependent destruction v0... inversion H.
+    - dependent destruction v; dependent destruction v0; inversion H.
+    - dependent destruction v; dependent destruction v0; inversion H.
     - f_equal; elim needy_to_term_injective with n n0; intros; subst...
-    - dependent destruction v... inversion H.
-    - dependent destruction v... inversion H.
-    - dependent destruction v; dependent destruction v0... inversion H.
-    - dependent destruction v; dependent destruction v0... inversion H.
-    - dependent destruction v... inversion H.
-    - dependent destruction v; dependent destruction v0... inversion H.
+    - dependent destruction v; inversion H.
+    - dependent destruction v; inversion H.
+    - dependent destruction v; dependent destruction v0; inversion H.
+    - dependent destruction v; dependent destruction v0; inversion H.
+    - dependent destruction v; inversion H.
+    - dependent destruction v; dependent destruction v0; inversion H.
       reflexivity.
-    - dependent destruction v; dependent destruction v0... inversion H.
-    - dependent destruction v; dependent destruction v0... inversion H.
-    - dependent destruction v; dependent destruction v0... inversion H.
-    - dependent destruction v... inversion H.
-    - dependent destruction v; dependent destruction v0... inversion H.
+    - dependent destruction v; dependent destruction v0; inversion H.
+    - dependent destruction v; dependent destruction v0; inversion H.
+    - dependent destruction v; dependent destruction v0; inversion H.
+    - dependent destruction v; inversion H.
+    - dependent destruction v; dependent destruction v0; inversion H.
     - dependent destruction v; dependent destruction v0;
       elim needy_to_term_injective with n n0; intros; subst; inversion H...
       rewrite <- H0; reflexivity.
   Qed.
 
-
-  (* Here comes the actual definition of the grammar of contexts. *)
-  (* We have two three non-trivial productions:  E -> E t,  E -> let x = t in E and *)
-  (* E -> let x := E in E[x] *)
-  (* There is also a trivial production  E -> [] which is omitted here. *)
-  (* The first parameter of eck is the nonterminal on the left-hand side; *)
-  (* the second parameter is the kind of the hole, i.e., the (unique) nonterminal *)
-  (* occurring on the right-hand side of a production. *)
-
-
-  (* N *)
+  (* E *)
   Inductive eck : ckind -> ckind -> Type :=
-  | eckApp : forall {m n}, term -> eck (ckv N m) (ckv N n)                   (* N -> N t *)
-  | eckSubst : forall {m n}, var -> term -> eck (ckv N m) (ckv N n)          (* N -> N[x / t] *)
-  | eckDist : forall {m n}, var -> var -> term -> eck (ckv N m) (ckv N n)    (* N -> N[x // λy.u] *)
-  | eckPlugSubst : forall {m n} x, needy x -> eck (ckv N m) (ckv N n).       (* N -> N<<x>>[x/N] *)
+  | eckApp : forall {k1 k2}, term -> eck k1 k2                (* E -> E t *)
+  | eckSubst : forall {k1 k2}, var -> term -> eck k1 k2       (* E -> E[x / t] *)
+  | eckDist : forall {k1 k2}, var -> var -> term -> eck k1 k2 (* E -> E[x // λy.u] *)
+  | eckPlugSubst : forall {k1 k2} x, needy x -> eck k1 k2.  (* E -> E<<x>>[x/E] *)
 
   Definition elem_context_kinded := eck.
   Hint Unfold elem_context_kinded.
 
   (* The starting symbol in the grammar *)
-  Definition init_ckind : ckind     :=  ckv N (Id 0).
+  Definition init_ckind : ckind :=  E.
 
   (* The function for plugging a term into an elementary context *)
   Definition elem_plug {k1 k2} (t : term) (ec : elem_context_kinded k1 k2) : term :=
-      match ec with
-      | eckApp t' => App t t'
-      | eckSubst x s => ExpSubst t x s
-      | eckDist x y u => ExpDist t x y u
-      | eckPlugSubst x n => ExpSubstS x n t
-      end.
-
-
-  (* Here we define substitution used in the definition of contraction. *)
+    match ec with
+    | eckApp t' => App t t'
+    | eckSubst x s => ExpSubst t x s
+    | eckDist x y u => ExpDist t x y u
+    | eckPlugSubst x n => ExpSubstS x n t
+    end.
 
   (* substitute term s for the needed variable x in the needy term n *)
   Fixpoint subst_needy (x : var) (n : needy x) (s : term) : term :=
@@ -477,18 +345,13 @@ Lemma sub_to_term_var_injective :
                                                    (*  again, types guarantee that x'=x *)
     | nExpSubst x' y _ n t => ExpSubst (subst_needy x' n s) y t
     | nExpSubstS x' y ny nx => ExpSubstS y ny (subst_needy x' nx s)
-
     | nExpDist x' y z _ nx t => ExpDist (subst_needy x' nx s) y z t
     end.
-
 
   (* Now we are ready to define the contraction. *)
   (* For the sake of simplicity we do not introduce the fourth (derived) rule *)
 
-  (*
-     Declares a set of nats using Coq.MSets.MSets.
-     Later this should be converted to a set of vars.
-   *)
+  (* Declares a set of nats using Coq.MSets.MSets. *)
   Module S := Make Nat_as_OT.
 
   Fixpoint fvn {x} (t : needy x) : S.t :=
@@ -517,38 +380,6 @@ Lemma sub_to_term_var_injective :
     | subDist l1 x y u => subDist (concat_sub l1 l2) x y u
     end.
 
-  (* Fixpoint fresh_var (t : term) : nat := *)
-  (*   match t with *)
-  (*   | Var (Id x) => x *)
-  (*   | Lam (Id x) p => max (fresh_var p) x *)
-  (*   | App p q => max (fresh_var p) (fresh_var q) *)
-  (*   | ExpSubst p (Id x) u => max (max (fresh_var p) (fresh_var u)) x *)
-  (*   | ExpSubstS (Id x) nx u => max (max (fresh_var u) (fresh_var (needy_to_term  nx))) x *)
-  (*   | ExpDist p (Id x) (Id y) u => max (max (max (fresh_var p) (fresh_var u)) y) x *)
-  (*   | ExpDistS (Id x) nx (Id y) u => max (max (max (fresh_var (needy_to_term nx)) (fresh_var u)) y) x *)
-  (*   end. *)
-
-  Fixpoint fresh_ind_n {x} (nx : needy x) : nat :=
-    match nx with
-    | nVar (Id x) => x
-    | nApp _ nx t => max (fresh_ind_n nx) (fresh_ind t)
-    | nExpSubst (Id x) (Id y) _ nx u => max (max (max (fresh_ind_n nx) (fresh_ind u)) y) x
-    | nExpSubstS (Id x) (Id y) nx ny => max (max (max (fresh_ind_n nx) (fresh_ind_n ny)) y) x
-    | nExpDist (Id x) (Id y) (Id z) _ nx u => max (max (max (max (fresh_ind_n nx) (fresh_ind u)) z) y) x
-    end
-  with fresh_ind (t : term) : nat :=
-    match t with
-    | Var (Id x) => x
-    | Lam (Id x) p => max (fresh_ind p) x
-    | App p q => max (fresh_ind p) (fresh_ind q)
-    | ExpSubst p (Id x) u => max (max (fresh_ind p) (fresh_ind u)) x
-    | ExpSubstS (Id x) nx u => max (max (fresh_ind u) (fresh_ind_n nx)) x
-    | ExpDist p (Id x) (Id y) u =>
-        max (max (fresh_ind p) (fresh_ind u)) (max x y)
-    | ExpDistS (Id x) nx (Id y) u =>
-        max (max (fresh_ind_n nx) (fresh_ind u)) (max x y)
-    end.
-
   Fixpoint skl_extract (t : term) (theta : S.t) (n : nat) : sub * term * nat :=
     if S.is_empty (S.inter theta (fv t)) then
       let x := Id n in
@@ -567,7 +398,6 @@ Lemma sub_to_term_var_injective :
              let '(l1, p', n') := skl_extract p (S.add x theta) n in
              let '(l2, u', m) := skl_extract u theta n' in
              (concat_sub l2 l1, ExpSubst p' (Id x) u', m)
-         (*DANIEL: extraction not acting on needy terms *)
          | ExpSubstS (Id x) nx u =>
              let '(l1, u', m) := skl_extract u theta n in
              (l1, ExpSubstS (Id x) nx u', m)
@@ -575,7 +405,6 @@ Lemma sub_to_term_var_injective :
              let '(l1, p', n') := skl_extract p (S.add x theta) n in
              let '(l2, u', m) := skl_extract u (S.add y theta) n' in
              (concat_sub l2 l1, ExpDist p' (Id x) (Id y) u', m)
-         (*DANIEL: extraction not acting on needy terms *)
          | ExpDistS (Id x) nx (Id y) u =>
              let '(l1, u', m) := skl_extract u (S.add y theta) n in
              (l1, ExpDistS (Id x) nx (Id y) u', m)
@@ -583,13 +412,10 @@ Lemma sub_to_term_var_injective :
 
   Definition contract {k} (r : redex k) : option term :=
       match r with
-      | rApp (vLam x t) l u => Some (ansCtx_plug (@sub_to_ansCtx k l) (ExpSubst t x u))
+      | rApp (vLam x t) l u => Some (sub_to_term l (ExpSubst t x u))
       | rSplS x nx (vLam (Id y) t) l =>
-          match k with
-          | @ckv _ (Id n) =>
-               let '(l', p', _) := skl_extract t (S.singleton y) n in
-               Some (sub_to_term l (sub_to_term l' (ExpDistS x nx (Id y) p')))
-          end
+           let '(l', p', _) := skl_extract t (S.singleton y) (1 + (fresh_ind t)) in
+           Some (sub_to_term l (sub_to_term l' (ExpDistS x nx (Id y) p')))
       | rSpl x nx t => Some (ExpSubstS x nx t)
       | rLsS x nx (vLam y p) => Some (ExpDist (subst_needy x nx (@vLam k y p)) x y p)
       | rLs x nx (vLam y p) => Some (ExpDistS x nx y p)
@@ -609,7 +435,6 @@ Lemma sub_to_term_var_injective :
     [ inversion H; trivial ].
   Qed.
 
-
   (* Next technicality: immediate_subterm has to be proved to be well-founded. *)
   (* Here we use a macro that does this for us. *)
   Lemma wf_immediate_subterm: well_founded immediate_subterm.
@@ -622,38 +447,35 @@ Lemma sub_to_term_var_injective :
 
 
   (* Decomposition of a value cannot give a potential redex, it must give a value. *)
-
-
-
   Lemma value_trivial1 :
     forall {k1 k2} (ec: elem_context_kinded k1 k2) t,
     forall v : value k1,  ec:[t] = v ->
                              exists (v' : value k2), t = v'.
   Proof with auto.
     intros ? ? ec t v H.
-    destruct ec; dependent destruction v; inversion H.
-    - try (dependent destruction s;
-      dependent destruction v; discriminate).
-    - destruct n0; try discriminate.
-      exists (ansNd x n0); inversion H; subst...
-    - dependent destruction s; dependent destruction v; try discriminate.
-      injection H1; intros; subst...
-      exists (ansVal (vLam v t1) s)...
-    - destruct n0; try discriminate.
-      injection H; intros; subst;
-      exists (ansNd _ n1); simpl; auto.
-    - dependent destruction s; dependent destruction v; try discriminate.
-      injection H1; intros; subst...
-      exists (ansVal (vLam v t1) s)...
-    - destruct n0; try discriminate.
-      injection H; intros; subst;
-      exists (ansNd _ n1); simpl; auto.
-    - dependent destruction s; dependent destruction v; try discriminate.
-    - destruct n1; try discriminate.
-      inversion H1; subst...
-      exists (ansNd _ n1_2)...
-  Qed.
+    destruct ec; dependent destruction v; inversion H;
+    destruct k2;
+    try (dependent destruction s;
+    dependent destruction v; discriminate).
+    destruct n; try discriminate.
+    exists (ansNd x n); inversion H; subst...
+    dependent destruction s; dependent destruction v; try discriminate.
+    injection H1; intros; subst...
+    exists (ansVal (vLam v t1) s)...
+    destruct n; try discriminate.
+    injection H; intros; subst;
+    exists (ansNd _ n0); simpl; auto.
+    dependent destruction s; dependent destruction v; try discriminate.
+    injection H1; intros; subst...
+    exists (ansVal (vLam v t1) s)...
+    destruct n; try discriminate.
+    injection H; intros; subst;
+    exists (ansNd _ n0); simpl; auto.
 
+    destruct n0; try discriminate.
+    inversion H1; subst...
+    exists (ansNd _ n0_2)...
+  Qed.
 
   (* A value is not a redex. *)
 
@@ -693,7 +515,7 @@ Lemma sub_to_term_var_injective :
       + dependent destruction v; dependent destruction v1; discriminate.
       + dependent destruction v. dependent destruction v2.
         inversion H. subst.
-        elim sub_plug_needy with s subEmpty (@vLam k v t) _ n...
+        elim sub_plug_needy with s subEmpty (@vLam E v t) _ n...
     - dependent destruction v0.
       destruct n0; try discriminate.
       inversion H1; subst.
@@ -704,22 +526,18 @@ Lemma sub_to_term_var_injective :
   (* there can be only values. *)
   Lemma redex_trivial1 :   forall {k k'} (r : redex k) (ec : elem_context_kinded k k') t,
        ec:[t] = r -> exists (v : value k'), t = v.
-
-  Proof with auto.
-      intros ? ? r ec t H.
-    destruct ec; dependent destruction r;
-    inversion H;
-    subst.
-    - exists (ansVal v s)...
-    - dependent destruction v.
-  Admitted.
-      (* exists (ansNd x n). *)
-    (* - exists (ansVal v l)... *)
-      (* exists (ansNd x n). *)
-    (* - exists (ansNd _ n)... *)
-    (* exists (ansVal v l)... *)
-  (* Qed. *)
-
+  Proof with eauto.
+    intros ? ? r ec t H.
+    destruct k; destruct k'; destruct ec;
+    dependent destruction r; inversion H;
+    destruct k;
+    try (destruct v; discriminate);
+    subst...
+    exists (ansVal v s)...
+    exists (ansNd _ n)...
+    destruct v; inversion H1; destruct k; exists (ansNd _ n)...
+    exists (ansVal v s)...
+  Qed.
 End Lam_cbnd_PreRefSem.
 
 
@@ -733,16 +551,17 @@ Module Lam_cbn_Strategy <: REF_STRATEGY Lam_cbnd_PreRefSem.
 
   (* Here is the down-arrow function. *)
   (* It is used to decompose a term.  *)
-
   Definition dec_term t k : elem_dec k :=
     match k with E =>
-                 match t with
-                 | App t1 t2 => ed_dec  E t1 (ap_r t2)
-                 | Var x     => ed_val (ansNd _ (nVar x))
-                 | Lam x t1  => ed_val (ansVal (vLam x t1) ansCtxEmpty)
-                 | Let x t1 t2 => ed_dec E t2 (in_let x t1)
-                 | LetS x t n => ed_dec E t (let_var x n)
-                 end
+      match t with
+      | App t1 t2 => ed_dec E t1 (eckApp t2)
+      | Var x     => ed_val (ansNd _ (nVar x))
+      | Lam x t1  => ed_val (ansVal (vLam x t1) subEmpty)
+      | ExpSubst t1 x t2 => ed_dec E t1 (eckSubst x t2)
+      | ExpSubstS x nx t => ed_dec E t (eckPlugSubst x nx)
+      | ExpDist t x y u => ed_dec E t (eckDist x y u)
+      | ExpDistS x nx y u => ed_red (rLsS x nx (vLam y u))
+      end
     end.
 
   (* The decomposed term after the decomposition must be equal *)
@@ -753,71 +572,92 @@ Module Lam_cbn_Strategy <: REF_STRATEGY Lam_cbnd_PreRefSem.
     destruct k,t ; simpl; auto.
   Qed.
 
-
   Definition dec_context {k k': ckind} (ec: elem_context_kinded k k') (v: value k') : elem_dec k :=
+  match k, k' with E, E =>
     match ec, v with
-    | ap_r t, ansVal v' s => ed_red  (rApp v' s t)
-    | ap_r t, ansNd _ n => ed_val (ansNd _ (nApp _ n t))
-    | in_let x t, ansVal v' s => ed_val (ansVal v' (ansCtxLet x t s))
-    | in_let x t, ansNd y n =>
+    | eckApp t, ansVal v' s => ed_red (rApp v' s t)
+    | eckApp t, ansNd _ n => ed_val (ansNd _ (nApp _ n t))
+    | eckSubst x t, ansVal v' s => ed_val (ansVal v' (subSubst s x t))
+    | eckDist x y u, ansVal v' s => ed_val (ansVal v' (subDist s x y u))
+    | eckSubst x t, ansNd y n =>
       (match eq_var y x with
-      | left peq => ed_red (rLet y t n) (* redex! *)
-      | right pneq => ed_val (ansNd y (nLet x _ pneq t n))
+      | left peq => ed_red (rSpl y n t) (* redex! *)
+      | right pneq => ed_val (ansNd y (nExpSubst y x pneq n t))
       end)
-    | let_var x n, ansVal v s => ed_red (rLetS _ n v s)
-    | let_var x n, ansNd _ n' => ed_val (ansNd _ (nLetS x _ n' n))
+    | eckDist x z u, ansNd y n =>
+      (match eq_var y x with
+      | left peq => ed_red (rLs y n (vLam z u)) (* redex! *)
+      | right pneq => ed_val (ansNd y (nExpDist y x z pneq n u))
+      end)
+    | eckPlugSubst x n, ansVal v s => ed_red (rSplS _ n v s)
+    | eckPlugSubst x n, ansNd _ n' => ed_val (ansNd _ (nExpSubstS _ x n n'))
+    end
+ end.
+
+  Ltac assert_by_proof_irrelevance :=
+    match goal with
+    | [ H : ?P, H1 : ?P |- _  ] => assert (H=H1) by apply proof_irrelevance
     end.
 
+  Ltac subst_proof_irrelevance := assert_by_proof_irrelevance; subst.
+  Ltac dep_subst_proof_irrelevance := assert_by_proof_irrelevance; dep_subst.
 
   (* The two pairs (term, context) before and after decomposition represent *)
   (* the same term. *)
-  Lemma dec_context_correct : forall {k k'} (ec : elem_context_kinded k k') (v : value k'),
-      ec:[v] = elem_rec (dec_context ec v).
-
+  Lemma dec_context_correct :
+    forall {k k'} (ec : elem_context_kinded k k') (v : value k'),
+    ec:[v] = elem_rec (dec_context ec v).
   Proof.
     intros ? ? ec v.
-    destruct ec; dependent destruction v;
-      simpl;
-      try solve [ auto ].
-    case_eq (eq_var x v0); intros; subst; auto.
+    destruct k; destruct k';
+    dependent destruction ec; dependent destruction v;
+    try destruct s;
+    try ( simpl; solve [ eauto ]); simpl.
+    - destruct v0; simpl; try reflexivity.
+      case_eq (eq_var x (Id n)); intros; subst; auto.
+    - destruct v1; simpl; try reflexivity.
+      case_eq (eq_var x (Id n)); intros; subst; auto.
   Qed.
-
 
   (* Here we define an order on elementary contexts but it is trivial in this case. *)
   Include Empty_search_order Lam_cbnd_PreRefSem.
 
   (* If two elementary contexts are prefixes of the same term, *)
   (* then they are equal. *)
-  Lemma search_order_comp_if :         forall t k k' k'' (ec0 : elem_context_kinded k k')
-                                                       (ec1 : elem_context_kinded k k''),
-      immediate_ec ec0 t -> immediate_ec ec1 t ->
-          k, t |~ ec0 << ec1  \/  k, t |~ ec1 << ec0  \/  (k' = k'' /\ ec0 ~= ec1).
-
+  Lemma search_order_comp_if :
+    forall t k k' k'' (ec0 : elem_context_kinded k k')
+      (ec1 : elem_context_kinded k k''),
+    immediate_ec ec0 t -> immediate_ec ec1 t ->
+      k, t |~ ec0 << ec1  \/  k, t |~ ec1 << ec0  \/  (k' = k'' /\ ec0 ~= ec1).
   Proof.
     intros t k k' k'' ec0  ec1 [? ?] [? ?].
     do 2 right.
     subst t.
     destruct ec0; dependent destruction ec1;
-    try discriminate;
-    injection H0; intros; subst; auto.
-    dependent destruction H.
-    auto.
+    destruct k0; destruct k1; destruct k2;
+    try discriminate.
+    - injection H0; intros; subst; split; auto.
+    - injection H0; intros; subst; split; auto.
+    - injection H0; intros; subst; split; auto.
+    - dependent destruction H0; split; auto.
   Qed.
 
+  Ltac prf := dep_subst_proof_irrelevance; try contradiction; try auto.
 
   (* Up-arrow function never returns that we should continue searching. *)
-  Lemma dec_context_term_next :                        forall {k0 k1 k2} (v : value k1) t
-                                                       (ec0 : elem_context_kinded k0 k1)
-                                                       (ec1 : elem_context_kinded k0 k2),
-      dec_context ec0 v = ed_dec _ t ec1 -> so_predecessor ec1 ec0 ec0:[v].
-
+  Lemma dec_context_term_next :
+    forall {k0 k1 k2} (v : value k1) t
+      (ec0 : elem_context_kinded k0 k1)
+      (ec1 : elem_context_kinded k0 k2),
+    dec_context ec0 v = ed_dec _ t ec1 -> so_predecessor ec1 ec0 ec0:[v].
   Proof.
-    intros ? ? ? v t ec0 ec1 H.
-    destruct ec0; dependent destruction ec1; dependent destruction v;
+    intros k0 k1 k2 v t ec0 ec1 H.
+    destruct k0; destruct k1; destruct k2.
+    destruct ec0; dependent destruction ec1;
+    dependent destruction v; destruct k1;
     try discriminate;
-    simpl in H; destruct (eq_var x v0); discriminate.
+    try (simpl in H; destruct (eq_var x v0); discriminate).
   Qed.
-
 End Lam_cbn_Strategy.
 
 
@@ -838,7 +678,7 @@ Require Import abstract_machine_facts.
 Module Lam_cbn_sim := DetAbstractMachine_Sim Lam_cbn_EAM.
 Import Lam_cbn_sim.
 
-
+(*TODO define some examples *)
 (* some terms for testing *)
 Definition x  := Id 1.
 Definition y  := Id 2.
